modules/verify/src/main/scala/specrest/verify/z3/SmtLib.scala
@@ -105,6 +105,8 @@ object SmtLib:
       s"(str.++ ${renderExpr(l)} ${renderExpr(r)})"
     case Z3Expr.SeqConcat(l, r, _) =>
       s"(seq.++ ${renderExpr(l)} ${renderExpr(r)})"
+    case Z3Expr.SeqContains(s, e, _) =>
+      s"(seq.contains ${renderExpr(s)} (seq.unit ${renderExpr(e)}))"
     case Z3Expr.Arith(op, args, _) =>
       s"(${ArithOp.token(op)} ${args.map(renderExpr).mkString(" ")})"
     case Z3Expr.Quantifier(q, bindings, body, _) =>
